LeanMqtt/Packets/VarHeader/Properties/Proofs.lean
@@ -12,7 +12,7 @@ open Mqtt
 
 theorem Properties.serialize_len (ps : Properties) :
     (Properties.serialize ps).length = GetByteSize.byteSize ps := by
-  exact SizedList.serialize_len ps VarInt.serialize_len
+  exact SizedList.serialize_len ps
 
 theorem Properties.roundtrip (ps : Properties) {rest : List UInt8} :
     Properties.parser.run (ps.serialize ++ rest) = some (ps, rest) :=
