LeanMqtt/Primitives/OptType/Proofs.lean
@@ -24,10 +24,20 @@ theorem OptType.reconstruct {α : Type} [c : Codec α] [LawfulCodec α]
     injection h_pair with _ _
 
 theorem OptType.serialize_len {α : Type} [Codec α] [GetByteSize α] {b : Bool}
-    (v : OptType α b) (h_len : ∀ a : α, (Codec.serialize a).length = GetByteSize.byteSize a) :
+    (v : OptType α b) [LawfulByteSize α] :
     (OptType.serialize b v).length = GetByteSize.byteSize v := by
   match b, v with
-  | true, val => exact h_len val
+  | true, val =>
+    exact @LawfulByteSize.serialize_len α _ _ _ val
   | false, () => rfl
+
+instance {α : Type} {b : Bool} [Codec α] [LawfulCodec α] : LawfulCodec (OptType α b) where
+  roundtrip := OptType.roundtrip b
+  reconstruct := OptType.reconstruct b
+
+instance {α : Type} {b : Bool}
+    [Codec α] [GetByteSize α] [LawfulCodec α] [LawfulByteSize α] :
+    LawfulByteSize (OptType α b) where
+  serialize_len := fun v => OptType.serialize_len v
 
 end Mqtt
